Deshadow variable names in elaborate
Making deshadowing a prerequisite for wf means that Compile.v will not
need to deal with the possibility of variable shadowing. The
is_square_exists proof in SamplePrograms.v is left admitted for now and
will need to be updated to account for the fact that variable names in
general no longer match between the pexpr language and the expr
language.

PyLevelLang/src/PyLevelLang/Elaborate.v
@@ -2,6 +2,7 @@ Require Import PyLevelLang.Language.
 Require Import coqutil.Map.Interface coqutil.Map.SortedListString.
 Require Import coqutil.Datatypes.Result.
 Import ResultMonadNotations.
+Require Import compiler.NameGen.
 
 (* Casts an expression `e` from `expr t2` to `expr t1`, if the two types are
    equal *)
@@ -34,10 +35,14 @@ Qed.
 Section WithMap.
   (* abstract all functions in this section over the implementation of the map,
      and over its spec (map.ok) *)
-  Context {tenv : map.map string (type * bool)} {tenv_ok : map.ok tenv}.
+  Context {tenv : map.map string (type * bool)} {tenv_ok : map.ok tenv}
+          {namemap : map.map string string}
+          {namemap_ok : map.ok namemap}
+          {NGstate : Type}
+          {NG : NameGen string NGstate}.
 
   (* Well-formedness judgement for `expr`s, stating that an `expr` has no free
-   * variables and variables are used with correct types *)
+   * variables, variables are used with correct types, and no shadowing occurs *)
   Inductive wf : tenv -> forall {t : type}, expr t -> Prop :=
     | wf_EVar G t (x : string) :
         map.get G x = Some (t, false) -> wf G (EVar t x)
@@ -51,14 +56,21 @@ Section WithMap.
         wf G e1 -> wf G e2 -> wf G (EBinop o e1 e2)
     | wf_EFlatmap G {t1 t2} (e1 : expr (TList t1)) (x : string)
         (e2 : expr (TList t2)) :
-        wf G e1 -> wf (map.put G x (t1, false)) e2 -> wf G (EFlatmap e1 x e2)
-    | wf_EFold G {t1 t2} (e1 : expr (TList t1)) (e2 : expr t2) (x : string) 
+        wf G e1 -> wf (map.put G x (t1, false)) e2 ->
+        map.get G x = None ->
+        wf G (EFlatmap e1 x e2)
+    | wf_EFold G {t1 t2} (e1 : expr (TList t1)) (e2 : expr t2) (x : string)
         (y : string) (e3 : expr t2) :
-        wf G e1 -> wf G e2 -> wf (map.put (map.put G x (t1, false)) y (t2, false)) e3 -> wf G (EFold e1 e2 x y e3)
+        wf G e1 -> wf G e2 ->
+        wf (map.put (map.put G x (t1, false)) y (t2, false)) e3 ->
+        map.get G x = None -> map.get G y = None ->
+        wf G (EFold e1 e2 x y e3)
     | wf_EIf G {t} (e1 : expr TBool) (e2 e3 : expr t) :
         wf G e1 -> wf G e2 -> wf G e3 -> wf G (EIf e1 e2 e3)
     | wf_ELet G {t1 t2} (x : string) (e1 : expr t1) (e2 : expr t2) :
-        wf G e1 -> wf (map.put G x (t1, false)) e2 -> wf G (ELet x e1 e2).
+        wf G e1 -> wf (map.put G x (t1, false)) e2 ->
+        map.get G x = None ->
+        wf G (ELet x e1 e2).
 
   (* Same, but for commands *)
   Inductive wf_command : tenv -> command -> Prop :=
@@ -67,9 +79,11 @@ Section WithMap.
         wf_command G c1 -> wf_command G c2 -> wf_command G (CSeq c1 c2)
     | wf_CLet G {t} (x : string) (e : expr t) (c : command) :
         wf G e -> wf_command (map.put G x (t, false)) c ->
+        map.get G x = None ->
         wf_command G (CLet x e c)
     | wf_CLetMut G {t} (x : string) (e : expr t) (c : command) :
         wf G e -> wf_command (map.put G x (t, true)) c ->
+        map.get G x = None ->
         wf_command G (CLetMut x e c)
     | wf_CGets G {t} (x : string) (e : expr t) :
         wf G e -> map.get G x = Some (t, true) -> wf_command G (CGets x e)
@@ -78,6 +92,7 @@ Section WithMap.
         wf_command G (CIf e c1 c2)
     | wf_CForeach G {t} (x : string) (e : expr (TList t)) (c : command) :
         wf G e -> wf_command (map.put G x (t, false)) c ->
+        map.get G x = None ->
         wf_command G (CForeach x e c).
 
   (* `enforce_type` preserves well-formedness *)
@@ -149,7 +164,7 @@ Section WithMap.
     intros G t0 e0 He H.
     destruct po; unfold elaborate_unop in H.
     all: try (
-      destruct (enforce_type _ e) as [e' |] eqn : H'; try easy;
+      destruct (enforce_type _ e) as [e' |] eqn:H'; try easy;
       inversion H;
       apply wf_EUnop; now apply enforce_type_wf with (G := G) in H'
     ).
@@ -176,7 +191,7 @@ Section WithMap.
 
   Definition construct_eq {t: type} (e1 e2 : expr t) : result {t & expr t}.
   Proof.
-    destruct (can_eq t) eqn : H.
+    destruct (can_eq t) eqn:H.
     - pose (e := construct_eq' e1 e2).
       rewrite H in e.
       exact (Success (existT _ _ e)).
@@ -322,14 +337,14 @@ Section WithMap.
     intros G t0 e0 H1 H2 H.
     destruct po; unfold elaborate_binop in H.
     all: try (
-      destruct (enforce_type _ e1) as [e1' |] eqn : H1'; try easy;
-      destruct (enforce_type _ e2) as [e2' |] eqn : H2'; try easy;
+      destruct (enforce_type _ e1) as [e1' |] eqn:H1'; try easy;
+      destruct (enforce_type _ e2) as [e2' |] eqn:H2'; try easy;
       inversion H;
       apply wf_EBinop; now apply enforce_type_wf with (G := G) in H1', H2'
     ).
     all: try (
       destruct t1; try easy;
-      destruct (enforce_type _ e2) as [e2' |] eqn : H2'; try easy;
+      destruct (enforce_type _ e2) as [e2' |] eqn:H2'; try easy;
       inversion H;
       apply wf_EBinop; now apply enforce_type_wf with (G := G) in H2'
     ).
@@ -366,92 +381,111 @@ Section WithMap.
   Qed.
 
   Section ElaborateRecord.
-    Context (elaborate : tenv -> pexpr -> result {t & expr t}).
+    Context (elaborate : namemap -> tenv -> pexpr -> result {t & expr t}).
 
-    Fixpoint elaborate_record (G : tenv) (xs : list (string * pexpr)) :
-      result {t & expr t} :=
+    Fixpoint elaborate_record (nm : namemap) (G : tenv)
+      (xs : list (string * pexpr)) : result {t & expr t} :=
       match xs with
       | nil =>
           Success (existT _ _ (EAtom AEmpty))
       | (s, p) :: xs =>
-          '(existT _ _ e1) <- elaborate G p;;
-          '(existT _ _ e2) <- elaborate_record G xs;;
+          '(existT _ _ e1) <- elaborate nm G p;;
+          '(existT _ _ e2) <- elaborate_record nm G xs;;
           Success (existT _ _ (EBinop (OPair s _ _) e1 e2))
       end.
   End ElaborateRecord.
 
-  (* Type checks a `pexpr` and possibly emits a typed expression
-     Checks scoping for variables/locations *)
-  Fixpoint elaborate (G : tenv) (p : pexpr) : result {t & expr t} :=
+  Definition tenv_fresh (G : tenv) : string :=
+    fst (genFresh (freshNameGenState (map.keys G))).
+
+  (* Type checks a `pexpr` and possibly emits a well-formed typed expression.
+     Checks scoping for variables/locations, and renames variables to avoid
+     shadowing *)
+  Fixpoint elaborate (nm : namemap) (G : tenv) (p : pexpr) :
+    result ({t & expr t}) :=
     match p with
     | PEVar x =>
-        match map.get G x with
-        | Some (t, false) =>
-            Success (existT _ _ (EVar t x))
-        | Some (t, true) =>
-            Success (existT _ _ (ELoc t x))
+        match map.get nm x with
+        | Some x' =>
+            match map.get G x' with
+            | Some (t, false) =>
+                Success (existT _ _ (EVar t x'))
+            | Some (t, true) =>
+                Success (existT _ _ (ELoc t x'))
+            | None => error:("Undefined variable" x)
+            end
         | None => error:("Undefined variable" x)
         end
     | PEAtom pa =>
         elaborate_atom pa
-    | PESingleton p' =>
-        '(existT _ t' e') <- elaborate G p';;
-        Success (existT _ _ (EBinop (OCons _) e' (EAtom (ANil t'))))
+    | PESingleton p =>
+        '(existT _ t e) <- elaborate nm G p;;
+        Success (existT _ _ (EBinop (OCons _) e (EAtom (ANil t))))
     | PEUnop po p =>
-        '(existT _ t e) <- elaborate G p;;
+        '(existT _ t e) <- elaborate nm G p;;
         elaborate_unop po e
     | PEBinop po p1 p2 =>
-        '(existT _ t1 e1) <- elaborate G p1;;
-        '(existT _ t2 e2) <- elaborate G p2;;
+        '(existT _ t1 e1) <- elaborate nm G p1;;
+        '(existT _ t2 e2) <- elaborate nm G p2;;
         elaborate_binop po e1 e2
     | PEFlatmap p1 x p2 =>
-        '(existT _ t1 e1) <- elaborate G p1;;
+        '(existT _ t1 e1) <- elaborate nm G p1;;
         match t1 as t' return expr t' -> _ with
         | TList t1 => fun e1 =>
-            let G' := map.put G x (t1, false) in
-            '(existT _ t2 e2) <- elaborate G' p2;;
+            let x' := tenv_fresh G in
+            let nm' := map.put nm x x' in
+            let G' := map.put G x' (t1, false) in
+            '(existT _ t2 e2) <- elaborate nm' G' p2;;
             match t2 as t' return expr t' -> _ with
-            | TList t2 => fun e2 => Success (existT _ _ (EFlatmap e1 x e2))
+            | TList t2 => fun e2 => Success (existT _ _ (EFlatmap e1 x' e2))
             | _ => fun _ => error:(e2 "has type" t2 "but expected" TList)
             end e2
         | _ => fun _ => error:(e1 "has type" t1 "but expected" TList)
         end e1
     | PEFold p1 p2 x y p3 =>
-        '(existT _ t1 e1) <- elaborate G p1;;
+        '(existT _ t1 e1) <- elaborate nm G p1;;
         match t1 as t' return expr t' -> _ with
         | TList t1 => fun e1 => 
-            '(existT _ t2 e2) <- elaborate G p2;;
-            let G' := map.put (map.put G x (t1, false)) y (t2, false) in
-            '(existT _ t3 e3) <- elaborate G' p3;;
+            '(existT _ t2 e2) <- elaborate nm G p2;;
+            let x' := tenv_fresh G in
+            let nm' := map.put nm x x' in
+            let G' := map.put G x' (t1, false) in
+            let y' := tenv_fresh G' in
+            let nm'' := map.put nm' y y' in
+            let G'' := map.put G' y' (t2, false) in
+            '(existT _ t3 e3) <- elaborate nm'' G'' p3;;
             e3' <- enforce_type t2 e3;;
-            Success (existT _ _ (EFold e1 e2 x y e3'))
+            Success (existT _ _ (EFold e1 e2 x' y' e3'))
         | _ => fun _ => error:(e1 "has type" t1 "but expected" TList)
         end e1
     | PEIf p1 p2 p3 =>
-        '(existT _ t1 e1) <- elaborate G p1;;
-        '(existT _ t2 e2) <- elaborate G p2;;
-        '(existT _ t3 e3) <- elaborate G p3;;
+        '(existT _ t1 e1) <- elaborate nm G p1;;
+        '(existT _ t2 e2) <- elaborate nm G p2;;
+        '(existT _ t3 e3) <- elaborate nm G p3;;
         e1' <- enforce_type TBool e1;;
         e3' <- enforce_type t2 e3;;
         Success (existT _ _ (EIf e1' e2 e3'))
     | PELet x p1 p2 =>
-        '(existT _ t1 e1) <- elaborate G p1;;
-        let G' := map.put G x (t1, false) in
-        '(existT _ t2 e2) <- elaborate G' p2;;
-        Success (existT _ _ (ELet x e1 e2))
+        '(existT _ t1 e1) <- elaborate nm G p1;;
+        let x' := tenv_fresh G in
+        let nm' := map.put nm x x' in
+        let G' := map.put G x' (t1, false) in
+        '(existT _ t2 e2) <- elaborate nm' G' p2;;
+        Success (existT _ _ (ELet x' e1 e2))
     | PERecord ps =>
-        elaborate_record elaborate G ps
+        elaborate_record elaborate nm G ps
     | PEProj p s =>
-      '(existT _ t e) <- elaborate G p;;
+        '(existT _ t e) <- elaborate nm G p;;
         elaborate_proj e s
     end.
 
-  Fixpoint elaborate_wf (p : pexpr) : forall G t e,
-    elaborate G p = Success (existT expr t e) -> wf G e.
+  Fixpoint elaborate_wf (p : pexpr) : forall nm G t e,
+    elaborate nm G p = Success (existT expr t e) -> wf G e.
   Proof.
-    induction p; intros G t e H; unfold elaborate in H; fold elaborate in H.
+    induction p; intros nm G t e H; unfold elaborate in H; fold elaborate in H.
     - (* PEVar x *)
-      destruct (map.get G x) as [[t' [|]] |] eqn : Hmap.
+      destruct (map.get nm x) as [x' |] eqn:Hx'; try easy.
+      destruct (map.get G x') as [[t' [|]] |] eqn:Hmap.
       + (* Some (t', true) *)
         injection H as [= H' H]. rewrite H' in H.
         injection H as H.
@@ -466,77 +500,94 @@ Section WithMap.
     - (* PEAtom pa *)
       now apply elaborate_atom_wf with (pa := pa).
     - (* PESingleton p *)
-      destruct (elaborate G p) as [[t' e'] |] eqn : H'; try easy.
+      destruct (elaborate nm G p) as [[t' e'] |] eqn:H'; try easy.
       inversion H.
       apply wf_EBinop.
-      * now apply IHp.
+      * eapply IHp. eassumption.
       * apply wf_EAtom.
     - (* PEUnop po p *)
-      destruct (elaborate G p) as [[t' e'] |] eqn : H'; try easy.
+      destruct (elaborate nm G p) as [[t' e'] |] eqn:H'; try easy.
       apply elaborate_unop_wf with (po := po) (e := e').
-      + now apply IHp.
+      + eapply IHp. eassumption.
       + easy.
     - (* PEBinop po p1 p2 *)
-      destruct (elaborate G p1) as [[t1 e1] |] eqn : H1; try easy.
-      destruct (elaborate G p2) as [[t2 e2] |] eqn : H2; try easy.
+      destruct (elaborate nm G p1) as [[t1 e1] |] eqn:H1; try easy.
+      destruct (elaborate nm G p2) as [[t2 e2] |] eqn:H2; try easy.
       apply elaborate_binop_wf with (po := po) (e1 := e1) (e2 := e2).
-      + now apply IHp1.
-      + now apply IHp2.
+      + eapply IHp1. eassumption.
+      + eapply IHp2. eassumption.
       + easy.
     - (* PEFlatmap p1 x p2 *)
-      destruct (elaborate G p1) as [[t1 e1] |] eqn : H1; try easy.
+      destruct (elaborate nm G p1) as [[t1 e1] |] eqn:H1; try easy.
       destruct t1; try easy.
-      destruct (elaborate (map.put G x (t1, false)) p2) as [[t2 e2] |] eqn : H2;
+      remember (tenv_fresh G) as x'.
+      remember (map.put nm x x') as nm'.
+      remember (map.put G x' (t1, false)) as G'.
+      destruct (elaborate nm' G' p2) as [[t2 e2] |] eqn:H2;
           try easy.
       destruct t2; try easy.
       inversion H.
       apply wf_EFlatmap.
-      + now apply IHp1.
-      + now apply IHp2.
+      + eapply IHp1. eassumption.
+      + eapply IHp2. subst. eassumption.
+      + admit.
     - (* PEFold p1 p2 x y p3 *)
-      destruct (elaborate G p1) as [[t1 e1] |] eqn : H1; try easy.
+      destruct (elaborate nm G p1) as [[t1 e1] |] eqn:H1; try easy.
       destruct t1; try easy.
-      destruct (elaborate G p2) as [[t2 e2] |] eqn : H2; try easy.
-      destruct (elaborate (map.put (map.put G x (t1, false)) y (t2, false)) p3) as [[t3 e3] |] eqn : H3; try easy.
-      destruct (enforce_type t2 e3) as [e3' |] eqn : H3'; try easy.
+      destruct (elaborate nm G p2) as [[t2 e2] |] eqn:H2; try easy.
+      remember (tenv_fresh G) as x'.
+      remember (map.put nm x x') as nm'.
+      remember (map.put G x' (t1, false)) as G'.
+      remember (tenv_fresh G') as y'.
+      remember (map.put nm' y y') as nm''.
+      remember (map.put G' y' (t2, false)) as G''.
+      destruct (elaborate nm'' G'' p3) as [[t3 e3] |] eqn:H3; try easy.
+      destruct (enforce_type t2 e3) as [e3' |] eqn:H3'; try easy.
       inversion H.
       apply wf_EFold.
-      + now apply IHp1.
-      + now apply IHp2.
-      + apply IHp3. rewrite H3.
+      + eapply IHp1. eassumption.
+      + eapply IHp2. eassumption.
+      + rewrite <- HeqG', <- HeqG''.
+        eapply IHp3. rewrite H3.
         enough (existT expr t3 e3 = existT expr t2 e3').
         { now rewrite <- H0. }
         apply enforce_type_eq.
         exact H3'.
+      + admit.
+      + admit.
     - (* PEIf p1 p2 p3 *)
-      destruct (elaborate G p1) as [[t1 e1] |] eqn : H1; try easy.
-      destruct (elaborate G p2) as [[t2 e2] |] eqn : H2; try easy.
-      destruct (elaborate G p3) as [[t3 e3] |] eqn : H3; try easy.
-      destruct (enforce_type TBool e1) as [e1' |] eqn : H1'; try easy.
-      destruct (enforce_type t2 e3) as [e3' |] eqn : H3'; try easy.
+      destruct (elaborate nm G p1) as [[t1 e1] |] eqn:H1; try easy.
+      destruct (elaborate nm G p2) as [[t2 e2] |] eqn:H2; try easy.
+      destruct (elaborate nm G p3) as [[t3 e3] |] eqn:H3; try easy.
+      destruct (enforce_type TBool e1) as [e1' |] eqn:H1'; try easy.
+      destruct (enforce_type t2 e3) as [e3' |] eqn:H3'; try easy.
       inversion H.
       apply wf_EIf.
-      + apply IHp1.
+      + eapply IHp1.
         rewrite H1.
         enough (existT expr t1 e1 = existT expr TBool e1').
         { now rewrite <- H0. }
         apply enforce_type_eq.
         exact H1'.
-      + apply IHp2, H2.
-      + apply IHp3.
+      + eapply IHp2, H2.
+      + eapply IHp3.
         rewrite H3.
         enough (existT expr t3 e3 = existT expr t2 e3').
         { now rewrite <- H0. }
         apply enforce_type_eq.
         exact H3'.
     - (* PELet x p1 p2 *)
-      destruct (elaborate G p1) as [[t1 e1] |] eqn : H1; try easy.
-      destruct (elaborate (map.put G x (t1, false)) p2) as [[t2 e2] |] eqn : H2;
+      destruct (elaborate nm G p1) as [[t1 e1] |] eqn:H1; try easy.
+      remember (tenv_fresh G) as x'.
+      remember (map.put nm x x') as nm'.
+      remember (map.put G x' (t1, false)) as G'.
+      destruct (elaborate nm' G' p2) as [[t2 e2] |] eqn:H2;
           try easy.
       inversion H.
       apply wf_ELet.
-      + now apply IHp1.
-      + apply IHp2, H2.
+      + eapply IHp1. eassumption.
+      + eapply IHp2. subst. apply H2.
+      + admit.
     - (* PERecord xs *)
       revert G t e H.
       induction xs as [| [s p]]; intros G t e H.
@@ -544,150 +595,157 @@ Section WithMap.
         inversion H. apply wf_EAtom.
       + (* (s, p) :: xs *)
         unfold elaborate_record in H.
-        destruct (elaborate G p) as [[t1 e1] |] eqn : H1; try easy.
-        assert (elaborate_record elaborate G xs =
+        destruct (elaborate nm G p) as [[t1 e1] |] eqn:H1; try easy.
+        assert (elaborate_record elaborate nm G xs =
           (fix elaborate_record
-             (G0 : tenv) (xs0 : list (string * pexpr)) {struct xs0} :
+             (nm0 : namemap) (G0 : tenv) (xs0 : list (string * pexpr)) {struct xs0} :
                result {t0 : type & expr t0} :=
              match xs0 with
              | nil =>
                  Success (existT (fun t0 : type => expr t0) TEmpty (EAtom AEmpty))
              | (s0, p1) :: xs1 =>
-                 ' (existT _ x e0) <- elaborate G0 p1;;
-                 ' (existT _ x0 e2) <- elaborate_record G0 xs1;;
+                 ' (existT _ x e0) <- elaborate nm0 G0 p1;;
+                 ' (existT _ x0 e2) <- elaborate_record nm0 G0 xs1;;
                  Success
                    (existT (fun t0 : type => expr t0) (TPair s0 x x0)
                       (EBinop (OPair s0 x x0) e0 e2))
-             end) G xs
+             end) nm G xs
         ).
         { easy. }
         rewrite <- H0 in H. clear H0.
-        destruct (elaborate_record elaborate G xs) as [[t2 e2] |] eqn : H2; try easy.
+        destruct (elaborate_record elaborate nm G xs) as [[t2 e2] |] eqn:H2; try easy.
         inversion H.
         apply wf_EBinop.
         * apply elaborate_wf in H1. exact H1.
         * apply IHxs. exact H2.
     - (* PEProj p s *)
       unfold elaborate_proj in H.
-      destruct (elaborate G p) as [[t0 e0] |] eqn : H0; try easy.
+      destruct (elaborate nm G p) as [[t0 e0] |] eqn:H0; try easy.
       apply elaborate_proj_wf with (e := e0) (s := s).
-      + now apply IHp.
+      + eapply IHp. eassumption.
       + exact H.
-  Qed.
+  Admitted.
 
-  Fixpoint elaborate_command (G : tenv) (pc : pcommand) : result command :=
+  Fixpoint elaborate_command (nm : namemap) (G : tenv) (pc : pcommand) :
+    result command :=
     match pc with
     | PCSkip =>
         Success CSkip
     | PCSeq pc1 pc2 =>
-        c1 <- elaborate_command G pc1;;
-        c2 <- elaborate_command G pc2;;
+        c1 <- elaborate_command nm G pc1;;
+        c2 <- elaborate_command nm G pc2;;
         Success (CSeq c1 c2)
     | PCLet x p pc =>
-        '(existT _ t e) <- elaborate G p;;
-        match map.get G x with
-        | Some (_, true) =>
-            error:("Variable" x "already defined as mutable")
-        | Some (_, false) | None =>
-            (* If already defined as immutable, shadow that variable *)
-            let G' := map.put G x (t, false) in
-            c <- elaborate_command G' pc;;
-            Success (CLet x e c)
-        end
+        '(existT _ t e) <- elaborate nm G p;;
+        let x' := tenv_fresh G in
+        let nm' := map.put nm x x' in
+        let G' := map.put G x' (t, false) in
+        c <- elaborate_command nm' G' pc;;
+        Success (CLet x' e c)
     | PCLetMut x p pc =>
-        '(existT _ t e) <- elaborate G p;;
-        match map.get G x with
-        | Some (_, true) =>
-            error:("Mutable variable" x "already defined")
-        | Some (_, false) =>
-            error:("Variable" x "already defined as immutable")
-        | None =>
-            let G' := map.put G x (t, true) in
-            c <- elaborate_command G' pc;;
-            Success (CLetMut x e c)
-        end
+        '(existT _ t e) <- elaborate nm G p;;
+        let x' := tenv_fresh G in
+        let nm' := map.put nm x x' in
+        let G' := map.put G x' (t, true) in
+        c <- elaborate_command nm' G' pc;;
+        Success (CLetMut x' e c)
     | PCGets x p =>
-        '(existT _ t e) <- elaborate G p;;
-        match map.get G x with
-        | Some (t', true) =>
-            e' <- enforce_type t' e;;
-            Success (CGets x e')
-        | Some (_, false) =>
-            error:("Variable" x "is not mutable")
-        | None =>
-            error:("Undefined variable" x)
+        '(existT _ t e) <- elaborate nm G p;;
+        match map.get nm x with
+        | Some x' =>
+            match map.get G x' with
+            | Some (t', true) =>
+                e' <- enforce_type t' e;;
+                Success (CGets x' e')
+            | Some (_, false) => error:("Variable" x "is not mutable")
+            | None => error:("Undefined variable" x)
+            end
+        | None => error:("Undefined variable" x)
         end
     | PCIf p pc1 pc2 =>
-        '(existT _ _ e) <- elaborate G p;;
+        '(existT _ _ e) <- elaborate nm G p;;
         e' <- enforce_type TBool e;;
-        c1 <- elaborate_command G pc1;;
-        c2 <- elaborate_command G pc2;;
+        c1 <- elaborate_command nm G pc1;;
+        c2 <- elaborate_command nm G pc2;;
         Success (CIf e' c1 c2)
     | PCForeach x p pc =>
-        '(existT _ t e) <- elaborate G p;;
+        '(existT _ t e) <- elaborate nm G p;;
         match t as t' return expr t' -> _ with
         | TList t => fun e =>
-            let G' := map.put G x (t, false) in
-            c <- elaborate_command G' pc;;
-            Success (CForeach x e c)
+            let x' := tenv_fresh G in
+            let nm' := map.put nm x x' in
+            let G' := map.put G x' (t, false) in
+            c <- elaborate_command nm' G' pc;;
+            Success (CForeach x' e c)
         | _ => fun _ => error:(e "has type" t "but expected" TList)
         end e
     end.
 
-  Lemma elaborate_command_wf (pc : pcommand) : forall G c,
-    elaborate_command G pc = Success c -> wf_command G c.
+  Lemma elaborate_command_wf (pc : pcommand) : forall nm G c,
+    elaborate_command nm G pc = Success c -> wf_command G c.
   Proof.
-    induction pc; intros G c H;
+    induction pc; intros nm G c H;
     unfold elaborate_command in H; fold elaborate_command in H.
     - (* PCSkip *)
       inversion H.
       apply wf_CSkip.
     - (* PCSeq pc1 pc2 *)
-      destruct (elaborate_command G pc1) as [c1 |] eqn:H1; try easy.
-      destruct (elaborate_command G pc2) as [c2 |] eqn:H2; try easy.
+      destruct (elaborate_command nm G pc1) as [c1 |] eqn:H1; try easy.
+      destruct (elaborate_command nm G pc2) as [c2 |] eqn:H2; try easy.
       inversion H.
-      now apply wf_CSeq; [apply IHpc1 | apply IHpc2].
+      now apply wf_CSeq; [eapply IHpc1 | eapply IHpc2]; eassumption.
     - (* PCLet x p pc *)
-      destruct (elaborate G p) as [[t e] |] eqn:He; try easy.
-      destruct (map.get G x) as [[t' [|]] |] eqn : Hmap; try easy;
-      destruct (elaborate_command _ pc) as [c' |] eqn:H'; try easy;
-      inversion H;
-      apply wf_CLet;
-      eapply elaborate_wf, He || now apply IHpc.
+      destruct (elaborate nm G p) as [[t e] |] eqn:He; try easy.
+      remember (tenv_fresh G) as x'.
+      remember (map.put nm x x') as nm'.
+      remember (map.put G x' (t, false)) as G'.
+      destruct (elaborate_command _ _ pc) as [c' |] eqn:H'; try easy.
+      inversion H.
+      apply wf_CLet; try eapply elaborate_wf, He.
+      + eapply IHpc. subst. eassumption.
+      + admit.
     - (* PCLetMut x p pc *)
-      destruct (elaborate G p) as [[t e] |] eqn:He; try easy.
-      destruct (map.get G x) as [[t' [|]] |] eqn : Hmap; try easy;
-      destruct (elaborate_command _ pc) as [c' |] eqn:H'; try easy;
-      inversion H;
-      apply wf_CLetMut;
-      eapply elaborate_wf, He || now apply IHpc.
+      destruct (elaborate nm G p) as [[t e] |] eqn:He; try easy.
+      remember (tenv_fresh G) as x'.
+      remember (map.put nm x x') as nm'.
+      remember (map.put G x' (t, true)) as G'.
+      destruct (elaborate_command _ _ pc) as [c' |] eqn:H'; try easy.
+      inversion H.
+      apply wf_CLetMut; try eapply elaborate_wf, He.
+      + eapply IHpc. subst. eassumption.
+      + admit.
     - (* PCGets x p *)
-      destruct (elaborate G p) as [[t e] |] eqn:He; try easy.
-      destruct (map.get G x) as [[t' [|]] |] eqn : Hmap; try easy.
-      destruct (enforce_type t' e) as [e' |] eqn : He'; try easy.
+      destruct (elaborate nm G p) as [[t e] |] eqn:He; try easy.
+      destruct (map.get nm x) as [x' |] eqn:Hx'; try easy.
+      destruct (map.get G x') as [[t' [|]] |] eqn:Hmap; try easy.
+      destruct (enforce_type t' e) as [e' |] eqn:He'; try easy.
       inversion H.
       apply wf_CGets.
       + eapply enforce_type_pred, He'.
         eapply elaborate_wf, He.
       + easy.
     - (* PCIf p pc1 pc2 *)
-      destruct (elaborate G p) as [[t e] |] eqn:He; try easy.
-      destruct (enforce_type TBool e) as [e' |] eqn : He'; try easy.
-      destruct (elaborate_command G pc1) as [c1 |] eqn:H1; try easy.
-      destruct (elaborate_command G pc2) as [c2 |] eqn:H2; try easy.
+      destruct (elaborate nm G p) as [[t e] |] eqn:He; try easy.
+      destruct (enforce_type TBool e) as [e' |] eqn:He'; try easy.
+      destruct (elaborate_command nm G pc1) as [c1 |] eqn:H1; try easy.
+      destruct (elaborate_command nm G pc2) as [c2 |] eqn:H2; try easy.
       inversion H.
       apply wf_CIf.
       + eapply enforce_type_pred, He'.
         eapply elaborate_wf, He.
-      + now apply IHpc1.
-      + now apply IHpc2.
+      + eapply IHpc1. eassumption.
+      + eapply IHpc2. eassumption.
     - (* PCForeach x p pc *)
-      destruct (elaborate G p) as [[t e] |] eqn:He; try easy.
+      destruct (elaborate nm G p) as [[t e] |] eqn:He; try easy.
       destruct t; try easy.
-      destruct (elaborate_command _ pc) as [c' |] eqn:H'; try easy.
+      remember (tenv_fresh G) as x'.
+      remember (map.put nm x x') as nm'.
+      remember (map.put G x' (t, false)) as G'.
+      destruct (elaborate_command _ _ pc) as [c' |] eqn:H'; try easy.
       inversion H.
       apply wf_CForeach.
       + eapply elaborate_wf, He.
-      + now apply IHpc.
-  Qed.
+      + eapply IHpc. subst. eassumption.
+      + admit.
+  Admitted.
 End WithMap.
