PyLevelLang/src/PyLevelLang/Examples.v
@@ -3,6 +3,7 @@ Require Import PyLevelLang.Elaborate.
 Require Import PyLevelLang.Interpret.
 Require Import coqutil.Map.Interface coqutil.Map.SortedListString coqutil.Map.Properties.
 Require Import coqutil.Datatypes.Result.
+Require Import compiler.NameGen compiler.StringNameGen.
 Import ResultMonadNotations.
 
 Section Examples.
@@ -15,8 +16,15 @@ Section Examples.
   Instance locals : map.map string {t & interp_type t} := SortedListString.map _.
   Instance locals_ok : map.ok locals := SortedListString.ok _.
 
+  Instance namemap : map.map string string := SortedListString.map _.
+  Instance namemap_ok : map.ok namemap := SortedListString.ok _.
+  Instance NG : NameGen string N := StringNameGen.
+
   Definition elaborate_interpret (l : locals) (p : pexpr) : result {t & interp_type t} :=
-    e <- elaborate (map.map_values (fun x => (projT1 x, true)) l) p;;
+    let G : tenv := map.map_values (fun x => (projT1 x, true)) l in
+    let vars := map.keys l in
+    let nm : namemap := map.of_list (List.zip pair vars vars) in
+    e <- elaborate nm G p;;
     Success (existT _ _ (interp_expr l (projT2 e))).
 
   Local Open Scope Z_scope.
@@ -27,7 +35,7 @@ Section Examples.
       (PEBinop POCons (PEAtom (PAInt 2))
         (PEBinop POCons (PEAtom (PAInt 3))
           (PESingleton (PEAtom (PAInt 4))))).
-  Goal elaborate map.empty ex1 =
+  Goal elaborate map.empty map.empty ex1 =
     Success (existT _ _
       (EBinop (OCons _) (EAtom (AInt 1))
         (EBinop (OCons _) (EAtom (AInt 2))
@@ -44,7 +52,7 @@ Section Examples.
       PEBinop POCons (PEAtom (PAInt 2)) (
         PEBinop POCons (PEAtom (PAInt 3)) (
           PESingleton (PEAtom (PAInt 4))))).
-  Goal elaborate map.empty ex2 = error:(
+  Goal elaborate map.empty map.empty ex2 = error:(
     (EBinop (OCons TInt) (EAtom (AInt 2))
       (EBinop (OCons TInt) (EAtom (AInt 3))
         (EBinop (OCons TInt) (EAtom (AInt 4))
@@ -68,20 +76,20 @@ Section Examples.
   Definition ex3 : pexpr :=
     PEProj (PELet "x" (PEAtom (PAInt 42))
       (PEBinop POPair (PEVar "x") (PEVar "x"))) "0".
-  Goal elaborate map.empty ex3 =
+  Goal exists x, elaborate map.empty map.empty ex3 =
     Success (existT _ _
-      (EUnop (OFst _ _ _) (ELet "x" (EAtom (AInt 42))
-        (EBinop (OPair "0" _ _) (EVar TInt "x")
-          (EBinop (OPair "1" _ _) (EVar TInt "x")
+      (EUnop (OFst _ _ _) (ELet x (EAtom (AInt 42))
+        (EBinop (OPair "0" _ _) (EVar TInt x)
+          (EBinop (OPair "1" _ _) (EVar TInt x)
             (EAtom AEmpty)))))).
-  reflexivity. Qed.
+  eexists. reflexivity. Qed.
   Goal elaborate_interpret map.empty ex3 = Success (existT _ TInt 42).
   reflexivity. Qed.
 
   Definition ex4 : pexpr :=
     PEProj (PELet "x" (PEAtom (PAInt 42))
       (PEBinop POPair (PEVar "x") (PEVar "y"))) "0".
-  Goal elaborate map.empty ex4 = error:("Undefined variable" "y").
+  Goal elaborate map.empty map.empty ex4 = error:("Undefined variable" "y").
   reflexivity. Qed.
   Goal elaborate_interpret map.empty ex4 = error:("Undefined variable" "y").
   reflexivity. Qed.
@@ -89,7 +97,7 @@ Section Examples.
   Definition ex5 : pexpr :=
     PEBinop POPair (PEAtom (PAInt 42))
       (PEBinop POPair (PEAtom (PABool true)) (PEAtom (PAString "hello"))).
-  Goal elaborate map.empty ex5 =
+  Goal elaborate map.empty map.empty ex5 =
     Success (existT _ _
       (EBinop (OPair "0" _ _) (EAtom (AInt 42))
         (EBinop (OPair "1" _ _)
@@ -115,7 +123,7 @@ Section Examples.
       :: ("string", PEAtom (PAString "abc"))
       :: ("int", PEAtom (PAInt (-2)))
       :: nil).
-  Goal elaborate map.empty ex6 =
+  Goal elaborate map.empty map.empty ex6 =
     Success (existT _ _
       (EBinop (OPair "bool" _ _) (EAtom (ABool false))
         (EBinop (OPair "string" _ _) (EAtom (AString "abc"))
@@ -136,7 +144,7 @@ Section Examples.
       :: ("b", PEAtom (PAInt 50))
       :: nil))
     "b".
-  Goal elaborate map.empty ex7 =
+  Goal elaborate map.empty map.empty ex7 =
     Success (existT _ _
       (EUnop (OFst _ _ _)
         (EUnop (OSnd _ _ _)
@@ -150,13 +158,13 @@ Section Examples.
 
   Definition ex8 : pexpr :=
     PEBinop POEq (PEAtom (PABool true)) (PEAtom (PAInt 5)).
-  Goal elaborate map.empty ex8 =
+  Goal elaborate map.empty map.empty ex8 =
     error:((EAtom (AInt 5)) "has type" TInt "but expected" TBool).
   reflexivity. Qed.
 
   Definition ex9 : pexpr :=
     PEBinop POEq (PEAtom (PABool true)) (PEAtom (PABool false)).
-  Goal elaborate map.empty ex9 =
+  Goal elaborate map.empty map.empty ex9 =
     Success (existT _ _
       (EBinop (OEq TBool eq_refl)
         (EAtom (ABool true)) (EAtom (ABool false)))).
